Tester accepts Apache

theories/Semantics.v
@@ -38,6 +38,22 @@ Inductive exp : Type -> Set :=
 | Exp__ETag  : var -> exp field_value
 | Exp__Match : field_value -> exp field_value -> exp bool.
 
+Fixpoint exp_to_sexp {T} (e : exp T) : sexp :=
+    match e with
+    | Exp__Const s    => [Atom "Constant string"; to_sexp s]
+    | Exp__Body  v    => [Atom "Message body"   ; to_sexp v]
+    | Exp__ETag  v    => [Atom "Entity tag"     ; to_sexp v]
+    | Exp__Match f fx => [Atom "Match tag"; to_sexp f; exp_to_sexp fx]
+    end%sexp.
+
+Instance Serialize__exp {T} : Serialize (exp T) :=
+  exp_to_sexp.
+
+Instance Serialize__resource : Serialize (resource_state exp) :=
+  fun r =>
+    let 'ResourceState b e := r in
+    [Atom "Resource"; to_sexp b; to_sexp e]%sexp.
+
 Notation connT := nat.
 
 Variant appE {exp_} : Type -> Type :=
@@ -45,13 +61,16 @@ Variant appE {exp_} : Type -> Type :=
 | App__Send : connT -> http_response exp_ -> appE unit.
 Arguments appE : clear implicits.
 
+Variant logE : Type -> Set :=
+  Log : string -> logE unit.
+
 Variant symE {exp_} : Type -> Set :=
   Sym__NewBody : symE (exp_ message_body)
 | Sym__NewETag : symE (exp_ field_value).
 Arguments symE : clear implicits.
 
-Class Is__smE E `{appE exp -< E} `{nondetE -< E} `{symE exp -< E}.
-Notation smE := (appE exp +' nondetE +' symE exp).
+Class Is__smE E `{appE exp -< E} `{nondetE -< E} `{logE -< E} `{symE exp -< E}.
+Notation smE := (appE exp +' nondetE +' logE +' symE exp).
 Instance smE_Is__smE : Is__smE smE. Defined.
 
 Definition http_smi {E R} `{Is__smE E} : itree E R :=
@@ -60,29 +79,37 @@ Definition http_smi {E R} `{Is__smE E} : itree E R :=
        '(c, Request (RequestLine methd t _) hs om) <- embed App__Recv st;;
        let send_code (sc : status_code) (b : option (exp message_body)) :=
            trigger (App__Send c (Response (status_line_of_code sc) [] b)) in
-       let ok (m : exp message_body)        := send_code 200 $ Some m in
-       let created     := send_code 201 None     in
-       let no_content  := send_code 204 None     in
-       let bad_request := send_code 400 None     in
-       let not_found   := send_code 404 None     in
+       let ok (m : exp message_body) := send_code 200 $ Some m in
+       let created     := send_code 201 None in
+       let no_content  := send_code 204 None in
+       let bad_request := send_code 400 None in
+       let wat {T} (mx : exp T) : exp message_body :=
+           match mx in exp _ with
+           | Exp__Const b => Exp__Const b
+           | Exp__Body  v => Exp__Body v
+           | Exp__ETag  _
+           | Exp__Match _ _ => Exp__Const ""
+           end in
+       let not_found :=
+           or (send_code 404 None)
+              (mx <- embed (@Sym__NewBody exp);;
+               send_code 404 (Some (wat mx)))in
        match t with
        | RequestTarget__Origin p _
        | RequestTarget__Absolute _ _ p _ =>
          match methd with
          | Method__GET =>
+           (* embed Log ("State before GET: " ++ to_string st);; *)
            match get p st with
            | Some (Some (ResourceState m _)) => ok m;; call st
-           | Some None => not_found;; call st
+           | Some None =>
+             (* embed Log (p ++ " is known as not found");; *)
+             not_found;; call st
            | None =>
+             (* embed Log (p ++ " is unknown");; *)
              or (not_found;; call (update p None st))
                 (mx <- embed (@Sym__NewBody exp);;
-                 let mx' : exp message_body :=
-                     match mx in exp message_body with
-                     | Exp__Const b => Exp__Const b
-                     | Exp__Body  v => Exp__Body v
-                     | Exp__ETag  _
-                     | Exp__Match _ _ => Exp__Const ""
-                     end in     (* WAT *)
+                 let mx' : exp message_body := wat mx in
                  ok mx';;
                  call (update p (Some (ResourceState mx' None)) st))
            end
@@ -90,6 +117,7 @@ Definition http_smi {E R} `{Is__smE E} : itree E R :=
          | Method__POST =>
            match om with
            | Some m =>
+             (* embed Log ("State before PUT: " ++ to_string st);; *)
              match get p st with
              | Some (Some _) => no_content
              | Some None     => created
@@ -102,4 +130,4 @@ Definition http_smi {E R} `{Is__smE E} : itree E R :=
            send_code 405 None;; call st
          end
        | _ => bad_request;; call st
-       end) [].
+       end)%string [].
